CrDsl.v
@@ -7,6 +7,7 @@ Import ListNotations.
 Require Import Strings.String.
 From MyProject Require Export CrIdentifiers.
 From MyProject Require Export CrTransformer.
+From MyProject Require Export ListUtils.
 
 (* A Module has a module name and either a parser or transformer definition *)
 Inductive Module : Type := 
@@ -17,4 +18,48 @@ Inductive Module : Type :=
 Inductive Connection : Type := 
   | ConnectionDef : ModuleName -> ModuleName -> ConnectionName -> Connection.
 
-Definition CaracaraProgram : Type := (list Module) * (list Connection).
+Inductive CaracaraProgram : Type := 
+  | CaracaraProgramDef : 
+      list ParserState -> 
+      list Header -> 
+      list StateVar -> 
+      list ModuleName -> 
+      list FunctionName -> 
+      list ConnectionName -> 
+      list CtrlPlaneConfigName -> 
+      list Module -> 
+      list Connection -> 
+      CaracaraProgram.
+
+Definition check_for_duplicate_identifiers (program : CaracaraProgram) : bool :=
+  match program with
+  | CaracaraProgramDef p h s m f c cc _ _ =>
+      has_duplicates (fun x y =>
+            match x, y with
+            | ParserStateCtr xid, ParserStateCtr yid => Nat.eqb xid yid
+            end) p ||
+      has_duplicates (fun x y =>
+            match x, y with
+            | HeaderCtr xid, HeaderCtr yid => Nat.eqb xid yid
+            end) h ||
+      has_duplicates (fun x y =>
+            match x, y with
+            | StateVarCtr xid, StateVarCtr yid => Nat.eqb xid yid
+            end) s ||
+      has_duplicates (fun x y =>
+            match x, y with
+            | ModuleNameCtr xid, ModuleNameCtr yid => Nat.eqb xid yid
+            end) m ||
+      has_duplicates (fun x y =>
+            match x, y with
+            | FunctionNameCtr xid, FunctionNameCtr yid => Nat.eqb xid yid
+            end) f ||
+      has_duplicates (fun x y =>
+            match x, y with
+            | ConnectionNameCtr xid, ConnectionNameCtr yid => Nat.eqb xid yid
+            end) c ||
+      has_duplicates (fun x y =>
+            match x, y with
+            | CtrlPlaneConfigNameCtr xid, CtrlPlaneConfigNameCtr yid => Nat.eqb xid yid
+            end) cc
+  end.
